src/go_lang/map.v
@@ -2,3 +2,5 @@ From Perennial.go_lang Require Export lang notation.
 From Perennial.go_lang Require Import typing.
 
 Definition NewMap {ext:ext_op} (t:ty) : expr := AllocMap (zero_val t).
+
+Definition mapT (vt:ty) : ty := refT (mapValT vt).
